\documentclass{article}
\usepackage{epsfig}
\pagestyle{empty}
\begin{document}
$ b^z = b^x + b^y $
\pagebreak

$ b^z = b^x(1 + b^{y-x}) = b^y(1 + e^{x-y}) $
\pagebreak

$ z = x + log_b(1 + b^{y-x}) = y + log_b(1 + b^{x-y}) $
\pagebreak

$ y > x, z = y + logadd\_table[-(x-y)] $
\pagebreak

$ x > y, z = x + logadd\_table[-(y-x)] $
\pagebreak

$ logadd\_table[n] = log_b(1 + b^{-n}) $
\pagebreak

$ log_b(2.0) $
\pagebreak

$ y = x $
\pagebreak

$ z = log_b(2x) = log_b(2) + x $
\pagebreak

$ log_b(x+y) = x = y $
\pagebreak

\end{document}
